theories/Syntax/Typ.v
@@ -1,16 +1,17 @@
-From Coq Require Import Classes.RelationClasses Classes.Morphisms Bool.Bool Classical_Prop.
+From Coq Require Import Classes.Morphisms Bool.Bool Classical_Prop.
 From DeBrLevel Require Import LevelInterface PairLevel.
 From Mecha Require Import Resource Resources.
 Import ResourceNotations ResourcesNotations SetNotations.
 
-(** * Syntax -  Type
+(** * Syntax - Type
 
- Based on the arrow-calculus, the set of types is endowed with a new 
- kind of arrow that represent signal functions. This new arrow carries 
- a set of resources used by this signal function.
-
+  Based on the arrow-calculus, the set of types is endowed with a new kind of arrow that represent signal functions. This new arrow carries a set of resources used by this signal function. Consequently, the definition of types relies on the module [Resources.v].
 *)
-Module Typ <: IsBdlLvlFullDTWL.
+
+(** ** Module - Type *)
+Module Typ <: IsBdlLvlDTWL.
+
+(** *** Definition *)
 
 Open Scope resource_scope.
 Open Scope set_scope.
@@ -18,341 +19,253 @@ Open Scope resources_scope.
 
 Module RS := Resources.
 
-(** *** Definition *)
+(** **** Type
 
-(** **** Type *)
+  A type is either a ground type, named [unit], a function type, a product type or a reactive type, also named signal function type. The first three type are usual in the extended lambda-calculus. The last one is a type taken from the arrow-calculus and represent reactive expressions. In addition, it carries a set of resource names representing interaction with the environment done by the expression.
+*)
 Inductive raw : Type :=
-  | ty_unit
-  | ty_arrow : raw -> raw -> raw
-  | ty_prod  : raw -> raw -> raw
-  | ty_reactive : raw -> raw -> resources -> raw
+  | ty_unit : raw
+  | ty_arrow (α β : raw) : raw
+  | ty_prod  (α β : raw) : raw
+  | ty_reactive (α β : raw) (R : resources) : raw
 .
 
 Definition t := raw.
-
-(** **** Equality *)
 Definition eq := @Logic.eq t.
-
-Fixpoint eqb' (τ τ' : t) : bool := 
-  match (τ,τ') with
-    | (ty_unit,ty_unit)                            => true
-    | (ty_prod τ1 τ2,ty_prod τ1' τ2')              => (eqb' τ1 τ1') && (eqb' τ2 τ2')
-    | (ty_arrow τ1 τ2,ty_arrow τ1' τ2')            => (eqb' τ1 τ1') && (eqb' τ2 τ2')
-    | (ty_reactive τ1 τ2 R,ty_reactive τ1' τ2' R') => (eqb' τ1 τ1') && (eqb' τ2 τ2') && 
-                                                      (R =? R')
-    | _ => false
-  end
-.
-
-Definition eqb := eqb'.
 
 (** **** Shift function 
 
-  The only elements that can be shift are sets on reactive arrow types.
+  The shift function impacts only the set of used resources. It takes a type goes through all sub-terms and applies the shift function defined for sets, in [Levels], on all used resource sets encountered.
 *)
-Fixpoint shift (lb : Lvl.t) (k : Lvl.t) (τ : t) : t := 
-  match τ with
+Fixpoint shift (lb : Lvl.t) (k : Lvl.t) (α : t) : t := 
+  match α with
     | ty_arrow t1 t2 => ty_arrow (shift lb k t1) (shift lb k t2)    
-    | ty_prod t1 t2 => ty_prod (shift lb k t1) (shift lb k t2)    
+    | ty_prod  t1 t2 => ty_prod  (shift lb k t1) (shift lb k t2)    
     | ty_reactive t1 t2 R => ty_reactive (shift lb k t1) (shift lb k t2) ([⧐ lb – k] R)
-    | _ => τ
+    | _ => α
   end
 .
 
-(** **** Multi shift 
+(** **** Multi shift function 
 
-During the functional transition, defined in [FT_Definition], the signal function is updated multiple 
-times with different lower bound and shift value. Thus, we define a [multi_shift] function that applies
-[n] shifts for two lists [lbs] and [ks] of length [n].
-
+  As done in [Resource.v] and [Resources.v], we define a [multi_shift] function that applies [n] shifts for two lists [lbs] and [ks] of length [n].
 *)
-Definition multi_shift (lbs : list nat) (ks : list nat) (t : t) :=
-  List.fold_right (fun (x : nat * nat) acc => let (lb,k) := x in shift lb k acc) t (List.combine lbs ks).
+Definition multi_shift (lbs : list lvl) (ks : list lvl) (α : t) :=
+  List.fold_right (fun lbk acc => shift (fst lbk) (snd lbk) acc) α (List.combine lbs ks).
 
 
 (** **** Valid function
 
-  In the same way than the [shift] function, the valid function scan the entire type and
-  verify the property if all carried sets satisfied the property of validity.
+  The well-formed property, named [valid], takes a level [k] called the well-formedness level and states that all resource names in the type are well-formed under [k]. Recall that a resource name [r] is well-formed under [k] if [r < k] and a resource set [s] is well-formed under [k] if all
+  [r] in [s] are well-formed under [k].
 *)
 Inductive valid' : Lvl.t -> t -> Prop :=
-  | vΤ_unit : forall k, valid' k ty_unit
-  | vΤ_prod : forall k τ1 τ2, valid' k τ1 -> valid' k τ2 -> valid' k (ty_prod τ1 τ2)
-  | vΤ_func : forall k τ1 τ2, valid' k τ1 -> valid' k τ2 -> valid' k (ty_arrow τ1 τ2)
-  | vΤ_reac : forall k τ1 τ2 R, valid' k τ1 -> valid' k τ2 -> k ⊩ R -> valid' k (ty_reactive τ1 τ2 R)
-.
-
-Fixpoint validb' (k : Lvl.t) (τ : t) :=
-  match τ with
-    | ty_unit => true
-    | ty_arrow t1 t2 =>  (validb' k t1) && (validb' k t2)   
-    | ty_prod t1 t2 =>  (validb' k t1) && (validb' k t2)   
-    | ty_reactive t1 t2 R =>  (validb' k t1) && (validb' k t2) && (k ⊩? R)
-  end
-.
+  | vΤ_unit (k : lvl): valid' k ty_unit
+  | vΤ_prod (k : lvl) (α β : t): valid' k α -> valid' k β -> valid' k (ty_prod α β)
+  | vΤ_func (k : lvl) (α β : t): valid' k α -> valid' k β -> valid' k (ty_arrow α β)
+  | vΤ_reac (k : lvl) (α β : t) (R : resources): 
+                   valid' k α -> valid' k β -> k ⊩ R -> valid' k (ty_reactive α β R).
 
 Definition valid := valid'.
-Definition validb := validb'.
 
-#[export]
-Hint Constructors valid' : core.
+#[export] Hint Constructors valid' : core.
 
-(** *** Equality *)
+(** *** Property *)
 
 #[export] Instance eq_refl : Reflexive eq := _.
 #[export] Instance eq_sym : Symmetric eq := _.
 #[export] Instance eq_trans : Transitive eq := _.
-
-#[export] 
-Hint Resolve eq_refl eq_sym eq_trans : core.
-
-#[export] Instance eq_rr : RewriteRelation eq := {}.
 #[export] Instance eq_equiv : Equivalence eq := _.
+#[export] Instance eq_rr : RewriteRelation eq := {}.
+#[export] Hint Resolve eq_refl eq_sym eq_trans : core.
 
-Lemma eqb_refl : forall τ, eqb τ τ = true.
+Lemma eq_dec (α β : t): {eq α β} + {~ eq α β}.
 Proof.
-  induction τ; simpl; auto; try (rewrite andb_true_iff; split; now auto).
-  repeat (rewrite andb_true_iff; split); auto. apply RS.St.eqb_refl.
-Qed.
-
-Lemma eqb_eq : forall τ1 τ2, eqb τ1 τ2 = true <-> eq τ1 τ2.
-Proof.
-  intros; split.
-  - revert τ2; unfold eq,eqb; induction τ1; intros; destruct τ2; inversion H; subst; auto.
-    -- apply andb_true_iff in H1 as [H1 H1']; f_equal; auto.
-    -- apply andb_true_iff in H1 as [H1 H1']; f_equal; auto.
-    -- apply andb_true_iff in H1 as [H1 H1'']; 
-        apply andb_true_iff in H1 as [H1 H1']; f_equal; auto.
-        apply RS.St.equal_spec in H1''; now apply RS.eq_leibniz.
-  - intros; rewrite H; apply eqb_refl.
-Qed.
-
-Lemma eqb_neq : forall τ τ', eqb τ τ' = false <-> ~ eq τ τ'.
-Proof.
-  split.
-  - unfold not; intros; apply eqb_eq in H0; rewrite H in *; inversion H0.
-  - rewrite <- eqb_eq; intros; now apply not_true_is_false.
-Qed.
-
-Lemma eq_dec : forall (τ τ' : t), {eq τ τ'} + {~ eq τ τ'}.
-Proof.
-  unfold eq; intros τ; induction τ; intros τ'; destruct τ'; simpl; auto; 
+  unfold eq; revert β; induction α; intro; destruct β; simpl; auto; 
   try (right; unfold not; intros contra; now inversion contra).
-  - destruct (IHτ1 τ'1); destruct (IHτ2 τ'2);
+  - destruct (IHα1 β1); destruct (IHα2 β2);
     try (right; unfold not; intros; inversion H; subst; contradiction); subst.
     f_equal; auto. 
-  - destruct (IHτ1 τ'1); destruct (IHτ2 τ'2);
+  - destruct (IHα1 β1); destruct (IHα2 β2);
     try (right; unfold not; intros; inversion H; subst; contradiction); subst.
     f_equal; auto.
-  - destruct (IHτ1 τ'1); destruct (IHτ2 τ'2); destruct (RS.eq_dec r r0);
+  - destruct (IHα1 β1); destruct (IHα2 β2); destruct (RS.eq_dec R R0);
     try (right; unfold not; intros; inversion H; subst; contradiction); subst.
     -- apply RS.eq_leibniz in e1; subst; auto.
     -- right; unfold not in *; intros; inversion H; subst; apply n; reflexivity.
 Qed.
 
-Lemma eq_dec' : forall (τ τ' : t), {τ = τ'} + {τ <> τ'}.
+Lemma eq_dec' (α β : t): {α = β} + {α <> β}.
+Proof. apply eq_dec. Qed.
+
+Lemma eq_leibniz (α β : t): eq α β -> α = β. 
+Proof. auto. Qed.
+
+(** **** [shift] property *)
+
+Lemma shift_zero_refl (k : lvl) (α : t):
+  (shift k 0 α) = α.
 Proof.
-  intros; destruct (eq_dec τ τ'). 
-  - unfold eq in *; subst; auto.
-  - unfold eq in *; auto.
-Qed.
-
-Lemma eq_leibniz : forall x y, eq x y -> x = y. Proof. auto. Qed.
-
-(** *** Shift *)
-
-Lemma shift_zero_refl : forall (lb : Lvl.t) (τ : t),
-  (shift lb 0 τ) = τ.
-Proof.
-  intros lb τ; induction τ; simpl; f_equal; auto.
+  induction α; simpl; f_equal; auto.
   apply RS.eq_leibniz; apply RS.shift_zero_refl.
 Qed.
 
-Lemma shift_valid_refl : forall lb k τ,
-  valid lb τ -> shift lb k τ = τ.
+Lemma shift_valid_refl (lb k : lvl) (α : t):
+  valid lb α -> shift lb k α = α.
 Proof.
-  intros; induction H; subst; simpl; f_equal; auto.
+  intro Hv; induction Hv; subst; simpl; f_equal; auto.
   apply RS.eq_leibniz; now apply RS.shift_valid_refl.
 Qed.
 
-#[export] Instance shift_eq : 
-  Proper (Logic.eq ==> Logic.eq ==> eq ==> eq) shift := _.
+#[export] Instance shift_eq : Proper (Logic.eq ==> Logic.eq ==> eq ==> eq) shift := _.
 
-Lemma shift_eq_iff : forall lb k τ τ1,
-  τ = τ1 <-> (shift lb k τ) = (shift lb k τ1).
+Lemma shift_eq_iff (lb k : lvl) (α β : t):
+  α = β <-> (shift lb k α) = (shift lb k β).
 Proof.
-  split.
-  - intros; now subst.
-  - revert τ1; induction τ; intros τ1' Heq; destruct τ1'; auto; 
+  split; intro Heq.
+  - now subst.
+  - revert β Heq; induction α; intros; destruct β; auto; 
     try (now inversion Heq); inversion Heq; f_equal; auto.
-    apply Resources.eq_leibniz. eapply Resources.shift_eq_iff.
+    apply Resources.eq_leibniz. 
+    eapply Resources.shift_eq_iff.
     now rewrite H2.
 Qed.
 
-Lemma shift_trans : forall lb k k' τ,
-  shift lb k (shift lb k' τ) = shift lb (k + k') τ.
+Lemma shift_trans (lb m n : lvl) (α : t):
+  shift lb m (shift lb n α) = shift lb (m + n) α.
 Proof.
-  intros; induction τ; simpl; f_equal; auto.
+  induction α; simpl; f_equal; auto.
   apply RS.eq_leibniz; apply RS.shift_trans.
 Qed.
 
-Lemma shift_permute : forall lb k k' τ,
-  shift lb k (shift lb k' τ) = shift lb k' (shift lb k τ).
+Lemma shift_permute (lb m n : lvl) (α : t):
+  shift lb m (shift lb n α) = shift lb n (shift lb m α).
 Proof.
-  intros; induction τ; simpl; f_equal; auto.
+  induction α; simpl; f_equal; auto.
   apply RS.eq_leibniz; apply RS.shift_permute.
 Qed.
 
-Lemma shift_permute_1 : forall t lb k k',
-  eq (shift lb k (shift lb k' t)) (shift (lb + k) k' (shift lb k t)).
+Lemma shift_permute_1 (lb m n : lvl) (α : t):
+  eq (shift lb m (shift lb n α)) (shift (lb + m) n (shift lb m α)).
 Proof.
-  unfold eq; intro t; induction t; intros; simpl; f_equal; auto.
+  unfold eq; induction α; intros; simpl; f_equal; auto.
   apply RS.eq_leibniz; apply RS.shift_permute_1.
 Qed.
 
-Lemma shift_permute_2 : forall t lb lb' k k',
-  lb <= lb' -> eq (shift lb k (shift lb' k' t)) (shift (lb' + k) k' (shift lb k t)).
+Lemma shift_permute_2 (lb k m n : lvl) (α : t):
+  lb <= k -> eq (shift lb m (shift k n α)) (shift (k + m) n (shift lb m α)).
 Proof.
-  unfold eq; intro t; induction t; intros; simpl; f_equal; auto.
+  unfold eq; induction α; intros; simpl; f_equal; auto.
   apply RS.eq_leibniz; now apply RS.shift_permute_2.
 Qed.
 
-Lemma shift_unfold : forall lb k k' t,
-  eq (shift lb (k + k') t) (shift (lb + k) k' (shift lb k t)). 
+Lemma shift_unfold (lb m n : lvl) (α : t):
+  eq (shift lb (m + n) α) (shift (lb + m) n (shift lb m α)). 
 Proof.
-  intros lb k k' t; induction t; simpl; auto.
-  - rewrite IHt1; rewrite IHt2; reflexivity.
-  - rewrite IHt1; rewrite IHt2; reflexivity.
-  - rewrite IHt1; rewrite IHt2. 
-    assert ([⧐ lb – k + k'] r = [⧐ lb + k – k'] [⧐ lb – k] r)%rs by apply Resources.shift_unfold.
-    apply RS.eq_leibniz in H; rewrite H; reflexivity.
+  induction α; simpl; auto; try now rewrite IHα1; rewrite IHα2.
+  rewrite IHα1; rewrite IHα2; unfold eq; f_equal. 
+  apply RS.eq_leibniz.
+  now apply RS.shift_unfold.
 Qed.
 
-Lemma shift_unfold_1 : forall k k' k'' t,
-  k <= k' -> k' <= k'' -> eq (shift k' (k'' - k') (shift k  (k' - k) t)) (shift k (k'' - k) t).
+Lemma shift_unfold_1 (k m n : lvl) (α : t):
+  k <= m -> m <= n -> eq (shift m (n - m) (shift k  (m - k) α)) (shift k (n - k) α).
 Proof.
-  intros k k' k'' t; induction t; simpl; intros; auto.
-  - rewrite IHt1; auto; rewrite IHt2; auto; reflexivity.
-  - rewrite IHt1; auto; rewrite IHt2; auto; reflexivity.
-  - rewrite IHt1; auto; rewrite IHt2; auto. 
-    assert ([⧐ k' – k'' - k'] [⧐ k – k' - k] r = [⧐ k – k'' - k] r )%rs.
-    -- apply RS.shift_unfold_1; auto.
-    -- apply RS.eq_leibniz in H1; rewrite H1; reflexivity.
+  induction α; simpl; intros Hlekm Hlemn; auto; 
+  try now rewrite IHα1; auto; rewrite IHα2; auto.
+  rewrite IHα1; auto; rewrite IHα2; auto; unfold eq; f_equal. 
+  apply RS.eq_leibniz.
+  now apply RS.shift_unfold_1.
 Qed.
 
-(** *** Valid *)
+(** **** [valid] property *)
 
-Lemma validb_valid : forall k t, validb k t = true <-> valid k t.
+#[export] Instance valid_eq : Proper (Logic.eq ==> eq ==> iff) valid := _.
+
+Lemma valid_weakening (k n : lvl) (α : t): (k <= n) -> valid k α -> valid n α.
 Proof.
-  intros k t; induction t; simpl; split; intros; auto.
-  - now constructor.
-  - rewrite andb_true_iff in *; destruct H; constructor; 
-    try (now rewrite <- IHt1); now rewrite <- IHt2.
-  - rewrite andb_true_iff in *; inversion H; subst; split; try (now rewrite IHt1);
-    now rewrite IHt2.
-  - rewrite andb_true_iff in *; destruct H; constructor; 
-    try (now rewrite <- IHt1); now rewrite <- IHt2.
-  - rewrite andb_true_iff in *; inversion H; subst; split; try (now rewrite IHt1);
-    now rewrite IHt2.
-  - repeat rewrite andb_true_iff in *; destruct H; destruct H; constructor;
-    try (now rewrite <- IHt1); try (now rewrite <- IHt2); now rewrite <- Resources.validb_valid.
-  - repeat rewrite andb_true_iff in *; inversion H; subst; repeat split; try (now rewrite IHt1);
-    try (now rewrite IHt2); now rewrite Resources.validb_valid.
+  unfold valid; induction α; intros Hleq Hvτ; simpl in *; inversion Hvτ; subst; eauto.
+  apply vΤ_reac; eauto. 
+  eapply RS.valid_weakening; eauto.
 Qed.
 
-Lemma validb_nvalid : forall k t, validb k t = false <-> ~ valid k t.
+Theorem shift_preserves_valid_1 (k m n : lvl) (α : t):
+  valid m α -> valid (m + n) (shift k n α).
 Proof.
-  intros; rewrite <- not_true_iff_false; split; intros; intro.
-  - apply H; now rewrite validb_valid. 
-  - apply H; now rewrite <- validb_valid.
+  unfold valid; induction α; intro Hvτ; inversion Hvτ; subst; simpl; auto.
+  apply vΤ_reac; auto. 
+  now apply RS.shift_preserves_valid_1.
 Qed.
 
-#[export] Instance valid_eq : 
-  Proper (Logic.eq ==> eq ==> iff) valid := _.
+Theorem shift_preserves_valid (m n : lvl) (α : t):
+  valid m α -> valid (m + n) (shift m n α).
+Proof. now apply shift_preserves_valid_1. Qed.
 
-#[export] Instance validb_eq : 
-  Proper (Logic.eq ==> eq ==> Logic.eq) validb := _.
-
-Lemma valid_weakening: forall k k' τ,
-  (k <= k') -> valid k τ -> valid k' τ.
-Proof.
-  unfold valid; intros k k' τ; induction τ; intros Hleq Hvτ; simpl in *;
-  inversion Hvτ; subst; eauto.
-  apply vΤ_reac; eauto. eapply RS.valid_weakening; eauto.
+Lemma shift_preserves_valid_zero (k : lvl) (α : t): valid k α -> valid k (shift k 0 α).
+Proof. 
+  intro Hvα; replace k with (k + 0) by auto. 
+  now apply shift_preserves_valid_1. 
 Qed.
 
-Theorem shift_preserves_valid_1 : forall lb k k' τ,
-  valid k τ -> valid (k + k') (shift lb k' τ).
+Lemma shift_preserves_valid_gen (lb k m n : lvl) (α : t):
+  m <= n -> lb <= k -> m <= lb -> n <= k -> n - m = k - lb -> 
+  valid lb α -> valid k (shift m (n - m) α).
 Proof.
-  unfold valid; intros lb k k' τ; induction τ; intro Hvτ; inversion Hvτ; subst; simpl; auto.
-  apply vΤ_reac; auto. now apply RS.shift_preserves_valid_1.
-Qed.
-
-Theorem shift_preserves_valid : forall k k' τ,
-  valid k τ -> valid (k + k') (shift k k' τ).
-Proof. intros; now apply shift_preserves_valid_1. Qed.
-
-Lemma shift_preserves_valid_zero : forall k t, valid k t -> valid k (shift k 0 t).
-Proof. intros; replace k with (k + 0); auto; now apply shift_preserves_valid_1. Qed.
-
-Lemma shift_preserves_valid_gen : forall lb lb' k k' t,
-  k <= k' -> lb <= lb' -> k <= lb -> k' <= lb' -> k' - k = lb' - lb -> 
-  valid lb t -> valid lb' (shift k (k' - k) t).
-Proof.
-  intros lb lb' k k' t; induction t; intros; simpl; inversion H4; subst; 
-  constructor; eauto; try (apply IHt1; now auto); try (apply IHt2; now auto).
+  intros Hlemn Hlelbk Hlemlb Hlenk Heq. 
+  induction α; intros; simpl; inversion H; subst; constructor; fold valid; auto. 
   apply RS.shift_preserves_valid_gen with lb; auto.
 Qed.
 
-Lemma shift_preserves_valid_2 : forall lb lb' t,
-  lb <= lb' -> valid lb t -> valid lb' (shift lb (lb' - lb) t).
-Proof. intros. eapply shift_preserves_valid_gen; eauto. Qed.
+Lemma shift_preserves_valid_2 (m n : lvl) (α : t):
+  m <= n -> valid m α -> valid n (shift m (n - m) α).
+Proof. intros Hle Hvα; eapply shift_preserves_valid_gen; eauto. Qed.
 
 End Typ.
 
+(** ---- *)
+
 (** * Syntax - Pair of types 
 
-  Resource context needs a pair of types. Knowing that the context
-  can be shifted, its elements need to implement shift, valid functions 
-  and their associated lemmas.
+  The resource context defined in [RContext.v] maps resource names to pair types. We define it co-domain here. Thanks to the [DeBrLevel] library, we do not have to prove properties that handle level because [PairLevel] already exists.
 *)
-Module PairTyp <: IsBdlLvlFullETWL := IsBdlLvlFullPairETWL Typ Typ.
 
-(** * Notation - Types *)
+
+(** ** Module - Pair of types *)
+Module PairTyp <: IsBdlLvlETWL := IsBdlLvlPairETWL Typ Typ.
+
+(** ---- *)
+
+(** ** Notation - Types *)
 Module TypNotations.
 
-(** ** Scope *)
+(** *** Scope *)
 Declare Scope typ_scope.
 Declare Scope ptyp_scope.
 Delimit Scope typ_scope with ty.
 Delimit Scope ptyp_scope with pty.
 
-(** ** Notations *)
+(** *** Notation *)
 Definition Τ := Typ.t.
 Definition πΤ := PairTyp.t.
   
 Notation "'𝟙'"       := Typ.ty_unit (in custom wh at level 0).
 Notation "T1 '→' T2" := (Typ.ty_arrow T1 T2) (in custom wh at level 50, right associativity).
-Notation "X '×' Y"   := (Typ.ty_prod X Y) (in custom wh at level 2, X custom wh, 
-                                              Y custom wh at level 0).
-Notation "τ1 '⟿' τ2 '∣' R" := (Typ.ty_reactive τ1 τ2 R) (in custom wh at level 50, 
-                                                             R constr, right associativity).
-Notation "'[⧐' lb '–' k ']' t" := (Typ.shift lb k t) (in custom wh at level 45, 
-                                                           right associativity) : typ_scope.
-Notation "'[⧐⧐' lb '–' k ']' t" := (Typ.multi_shift lb k t) (in custom wh at level 45, 
-right associativity) : typ_scope.
-Notation "'[⧐' lb '–' k ']' t" := (PairTyp.shift lb k t) (in custom wh at level 45, 
-right associativity) : ptyp_scope.
+Notation "X '×' Y"   := (Typ.ty_prod X Y) 
+                        (in custom wh at level 2, X custom wh, Y custom wh at level 0).
+Notation "α '⟿' β '∣' R" := (Typ.ty_reactive α β R)
+                               (in custom wh at level 50, R constr, right associativity).
+Notation "'[⧐' lb '–' k ']' t" := (Typ.shift lb k t) 
+                                   (in custom wh at level 45, right associativity) : typ_scope.
+Notation "'[⧐⧐' lb '–' k ']' t" := (Typ.multi_shift lb k t) 
+                                    (in custom wh at level 45, right associativity) : typ_scope.
+Notation "'[⧐' lb '–' k ']' t" := (PairTyp.shift lb k t) 
+                                   (in custom wh at level 45, right associativity) : ptyp_scope.
 
-Infix "⊩"   := Typ.valid (at level 20, no associativity): typ_scope. 
-Infix "⊩?"  := Typ.validb (at level 20, no associativity) : typ_scope. 
+Infix "⊩"  := Typ.valid (at level 20, no associativity): typ_scope. 
 Infix "⊩"  := PairTyp.valid (at level 20, no associativity) : ptyp_scope. 
-Infix "⊩?" := PairTyp.validb (at level 20, no associativity) : ptyp_scope. 
-
 Infix "="  := Typ.eq : typ_scope.
-Infix "=?" := Typ.eqb  (at level 70) : typ_scope.
 
-(** ** Morphism *)
+(** *** Morphism *)
 #[export] Instance typ_leibniz_eq : Proper Logic.eq Typ.eq := _.
 
 End TypNotations.
