theories/Syntax/Var.v
@@ -5,22 +5,31 @@ From DeBrLevel Require Import LevelInterface.
 
   We represent variables with [nat]. 
 *)
+
+(** ** Module - Variable *)
 Module Var <: OrderedTypeWithLeibniz.
+
+(** *** Definition *)
 
 Include Nat_as_OT.
 
-Lemma eq_leibniz : forall x y, eq x y -> x = y. Proof. auto. Qed.
+(** *** Property *)
+
+Lemma eq_leibniz (x y : t): eq x y -> x = y. 
+Proof. auto. Qed.
 
 End Var.
 
-(** * Notation - Variable *)
+(** ---- *)
+
+(** ** Notation - Variable *)
 Module VarNotations.
 
-(** ** Scope *)
+(** *** Scope *)
 Declare Scope var_scope.
 Delimit Scope var_scope with v.
 
-(** ** Notations *)
+(** *** Notation *)
 Definition variable := Var.t.
 
 Infix "<"  := Var.lt : var_scope.
@@ -28,7 +37,7 @@ Infix "="  := Var.eq : var_scope.
 Infix "<?" := Var.ltb (at level 70) : var_scope.
 Infix "=?" := Var.eqb (at level 70) : var_scope.
 
-(** ** Morphism *)
+(** *** Morphism *)
 #[export] Hint Resolve Var.eq_refl Var.eq_sym Var.eq_trans : core.
 #[export] Instance var_eq_rr : RewriteRelation Var.eq := _.
 #[export] Instance var_eq_equiv : Equivalence Var.eq := _.
